VST-introduction/Spec_kalloc.v
@@ -11,13 +11,13 @@ Global Open Scope funspec_scope.
 (******************************)
 
 (*** kalloc token type... *)
-Definition my_kalloc_token {cs: compspecs} sh t p :=
+Definition my_kalloc_token K {cs: compspecs} sh t p :=
   !! field_compatible t [] p && (* this shoudl work because of memory_block_data_at_*)
-  (kalloc_token_sz sh (sizeof t) p).
+  (kalloc_token' K sh (sizeof t) p).
 
 Lemma my_kalloc_token_valid_pointer:
-  forall (sh : share) (t : type) (p : val),
-  my_kalloc_token sh t p |-- valid_pointer p.
+  forall K (sh : share) (t : type) (p : val),
+  my_kalloc_token K sh t p |-- valid_pointer p.
 Proof.
   intros. 
   unfold my_kalloc_token. unfold kalloc_token_sz. entailer!.
@@ -45,23 +45,23 @@ Ltac kalloc_token_data_at_valid_pointer :=
   (simple apply my_kalloc_token_valid_pointer; data_at_valid_aux) : valid_pointer.
 #[export] Hint Extern 4 (_ |-- valid_pointer _) => kalloc_token_data_at_valid_pointer : valid_pointer.
 
-Lemma my_kalloc_token_local_facts:  forall {cs: compspecs} sh t p,
-      my_kalloc_token sh t p |-- !! (field_compatible t [] p /\ malloc_compatible (sizeof t) p).
+Lemma my_kalloc_token_local_facts: forall K {cs: compspecs} sh t p,
+      my_kalloc_token K sh t p |-- !! (field_compatible t [] p /\ malloc_compatible (sizeof t) p).
 Proof. intros.
  unfold my_kalloc_token.
  normalize. rewrite prop_and.
  apply andp_right. apply prop_right; auto.
- apply kalloc_token_sz_local_facts.
+ apply kalloc_token'_local_facts.
 Qed.
 #[export] Hint Resolve my_kalloc_token_local_facts : saturate_local.
 
 
 Lemma my_kalloc_token_split: 
- forall (sh: share) (t: type) (p: val),
- my_kalloc_token (sh) (t) (p)
+ forall K (sh: share) (t: type) (p: val),
+ my_kalloc_token K (sh) (t) (p)
   = 
   !! field_compatible t [] p &&
-  (kalloc_token_sz sh (sizeof t) p).
+  (kalloc_token' K sh (sizeof t) p).
 Proof.
   intros. apply pred_ext.
   - unfold my_kalloc_token. entailer.
@@ -80,7 +80,7 @@ Definition kfree1_spec (K:KallocFreeAPD) {cs: compspecs} (t: type) :=
         SEP (
           ASI_kalloc.mem_mgr K gv sh ls xx original_freelist_pointer;
           if eq_dec new_head nullval then emp
-          else (my_kalloc_token sh (t) new_head (* data_at_ Ews t new_head*))
+          else (my_kalloc_token K sh (t) new_head (* data_at_ Ews t new_head*))
         )
       POST [ tvoid ]
         PROP()
@@ -94,9 +94,9 @@ Definition kfree1_spec (K:KallocFreeAPD) {cs: compspecs} (t: type) :=
 
 Definition kalloc1_spec (K:KallocFreeAPD) {cs: compspecs} (t: type) :=
 DECLARE _kalloc1
-WITH n:Z, gv:globals, sh:share, ls: list val, xx:Z, original_freelist_pointer:val
+WITH gv:globals, sh:share, ls: list val, xx:Z, original_freelist_pointer:val
 PRE [ ]
-    PROP(0 <= n <= PGSIZE;
+    PROP(0 <= (sizeof t) <= PGSIZE;
             complete_legal_cosu_type t = true;
             natural_aligned natural_alignment t = true) 
     PARAMS () GLOBALS(gv)
@@ -106,37 +106,45 @@ POST [ tptr tvoid ]
     RETURN (original_freelist_pointer) 
     SEP (
       if (eq_dec original_freelist_pointer nullval) then
-      ASI_kalloc.mem_mgr K gv sh ls xx original_freelist_pointer * emp
+        (ASI_kalloc.mem_mgr K gv sh ls xx original_freelist_pointer * emp)
       else 
         (
           EX next ls',
           (!! (next :: ls' = ls) &&
-              my_kalloc_token sh t original_freelist_pointer *
+              my_kalloc_token K sh t original_freelist_pointer *
               ASI_kalloc.mem_mgr K gv sh ls' xx next
         )
         )
     ).
 
-  Lemma kalloc1_spec_sub:
-    forall  (K:KallocFreeAPD) {cs: compspecs} (t: type), 
-      funspec_sub (snd (kalloc1_spec_sz K _kalloc1)) (snd (kalloc1_spec K t)).
-   Proof.
-     do_funspec_sub. 
+
+
+Lemma kalloc1_spec_sub:
+  forall  (K:KallocFreeAPD) {cs: compspecs} (t: type), 
+    funspec_sub (snd (kalloc1_spec' K _kalloc1)) (snd (kalloc1_spec K t)).
+  Proof.
+    do_funspec_sub. 
+    entailer.
+    destruct w.
+    repeat (destruct p).
+    Exists (sizeof t, g0, s, l, z, v) emp. entailer.
+    if_tac.
+    (*entailer.
+    destruct (EqDec_val v nullval).*)
+    - entailer!. entailer!. (*split.
+      + entailer!.
+      + admit. (* assume sizeof t can fit within the pgsize.. *)*)
+    - entailer!. (*split.*)
+      + entailer!. Exists next ls'. entailer!. unfold my_kalloc_token. 
+      assert_PROP (field_compatible t [] (eval_id ret_temp x)).
+      { entailer!.
+        apply malloc_compatible_field_compatible; auto. }
       entailer.
-      Exists w emp. entailer.
-      repeat destruct w.
-      repeat destruct p.
-      entailer.
-      entailer!. intros. destruct (EqDec_val (eval_id ret_temp x) nullval).
-      entailer!.
-      Intros next ls'. Exists next ls'.
-      entailer!.
-      admit.
-Admitted.
+Qed.
 
 Lemma kfree1_spec_sub:
-forall  (K:KallocFreeAPD) {cs: compspecs} (t: type), (* TODO: fix: this is not general, but it uses KF_APD *)
-  funspec_sub (snd (kfree1_spec_sz KF_APD _kfree1)) (snd (kfree1_spec KF_APD t)).
+forall  (K:KallocFreeAPD) {cs: compspecs} (t: type), 
+  funspec_sub (snd (kfree1_spec' K _kfree1)) (snd (kfree1_spec K t)).
 Proof.
   do_funspec_sub. 
   destruct w.
