VST-introduction/VSU_kalloc_kfree_definitions.v
@@ -7,7 +7,6 @@ Require Import malloc_sep.*)
 
 (* THIS SHOULD CONTAIN ANY INTERNAL FUNCTIONS... I DON'T HAVE ANY *)
 
-
 Definition kalloc_token_sz (sh: share) (n: Z) (p: val) : mpred :=
   !! ((*field_compatible t_run [] p /\*)
       0 < n <= PGSIZE
@@ -32,8 +31,24 @@ Proof.
   intros. 
   unfold kalloc_token_sz. simpl. entailer.
 Qed.
-(***** kalloc token size ******)
 
+Lemma kalloc_token_sz_split:
+forall  (sh: share) (n: Z) (p: val),
+  kalloc_token_sz sh n p =
+  !! ((*field_compatible t_run [] p /\*)
+  0 < n <= PGSIZE
+  /\ malloc_compatible (n) p 
+  /\ malloc_compatible (PGSIZE) p
+  /\ writable_share sh
+  (*/\  maybe some alignment and physical address checks here *))
+  && memory_block sh (n) (p).
+Proof.
+  intros. apply pred_ext.
+  - unfold kalloc_token_sz. entailer.
+  - unfold kalloc_token_sz. entailer!.
+Qed.
+
+(***** kalloc token size ******)
 
 Definition Tok_APD := Build_KallocTokenAPD kalloc_token_sz kalloc_token_sz_valid_pointer
   kalloc_token_sz_local_facts.
@@ -64,22 +79,6 @@ Proof.
   intros. apply pred_ext.
   - unfold mem_mgr. entailer!.
   - unfold mem_mgr. entailer!.
-Qed.
-
-Lemma kalloc_token_sz_split:
-forall  (sh: share) (n: Z) (p: val),
-  kalloc_token_sz sh n p =
-  !! ((*field_compatible t_run [] p /\*)
-  0 < n <= PGSIZE
-  /\ malloc_compatible (n) p 
-  /\ malloc_compatible (PGSIZE) p
-  /\ writable_share sh
-  (*/\  maybe some alignment and physical address checks here *))
-  && memory_block sh (n) (p).
-Proof.
-  intros. apply pred_ext.
-  - unfold kalloc_token_sz. entailer.
-  - unfold kalloc_token_sz. entailer!.
 Qed.
 
 (************ lemmas etc. end *************)
