VST-introduction/verif_kalloc1_kfree1.v
@@ -14,7 +14,7 @@ Require Import malloc_lemmas.
 Require Import malloc_sep.*)
 Require Import VC.VSU_kalloc_kfree_definitions.
 
-Lemma body_kfree1 i: semax_body MF_Vprog MF_Gprog f_kfree1 (kfree1_spec_sz KF_APD i).
+Lemma body_kfree1: semax_body MF_Vprog MF_Gprog f_kfree1 (kfree1_spec KF_APD t_run).
 Proof. start_function. Intros.
 forward.
 rewrite mem_mgr_split. Intros.
@@ -23,16 +23,19 @@ destruct (eq_dec new_head nullval).
     * rewrite e in H2; auto_contradict.
     * forward. entailer. rewrite mem_mgr_split. entailer.
 - forward_if.
-    * Intros. forward. intros. rewrite kalloc_token_sz_split. Intros.
+    * Intros. forward. unfold my_kalloc_token. Intros. rewrite kalloc_token_sz_split. Intros. 
+    rewrite memory_block_data_at_; auto. forward. forward. 
+    (*forward. intros. rewrite kalloc_token_sz_split. Intros.
     rewrite memory_block_data_at_.
-     forward.
+     forward.*) entailer. rewrite mem_mgr_split. refold_freelistrep. entailer!.
+     right; split; auto. unfold not; auto_contradict.
     * forward. entailer.
-Admitted.
+Qed.
 
 
-Lemma body_kalloc1 i: semax_body MF_Vprog MF_Gprog f_kalloc1 (kalloc1_spec (KF_APD) i).
+Lemma body_kalloc1: semax_body MF_Vprog MF_Gprog f_kalloc1 (kalloc1_spec (KF_APD) t_run).
 Proof. start_function.
-rewrite mem_mgr_split. Intros. forward.  unfold abbreviate in POSTCONDITION.
+rewrite mem_mgr_split. Intros. forward.  (*unfold abbreviate in POSTCONDITION.*)
 forward_if (
     PROP  ( )
     LOCAL (
@@ -40,26 +43,45 @@ forward_if (
         gvars gv
         )
     SEP (
-        ASI_kalloc.mem_mgr KF_APD gv sh ls xx original_freelist_pointer*
+        if (eq_dec original_freelist_pointer nullval) then
+        (ASI_kalloc.mem_mgr KF_APD gv sh ls xx original_freelist_pointer * emp)
+      else 
+        (
+          EX next ls',
+          (!! (next :: ls' = ls) &&
+              my_kalloc_token KF_APD sh (t_run) original_freelist_pointer *
+              ASI_kalloc.mem_mgr KF_APD gv sh ls' xx next
+          )
+        )
+        (*ASI_kalloc.mem_mgr KF_APD gv sh ls xx original_freelist_pointer*
                    (if eq_dec original_freelist_pointer nullval
                    then emp
-                   else kalloc_token' KF_APD sh PGSIZE original_freelist_pointer)
+                   else my_kalloc_token KF_APD sh t_run original_freelist_pointer)*)
     )
 )%assert.
-+forward. destruct H0 as [[H0011 H0012] | [H0021 H0022]].
-    - rewrite H0012 in H1; auto_contradict.
-    - destruct ls; auto_contradict.
+- destruct H3 as [[H0011 H0012] | [H0021 H0022]].
+    + rewrite H0012 in H4; auto_contradict.
+    + destruct ls; auto_contradict.
     refold_freelistrep. Intros.
-    forward. forward.
-    destruct (eq_dec original_freelist_pointer nullval) eqn:e1; auto_contradict. entailer.
-    rewrite mem_mgr_split. Exists sh (v::ls) xx original_freelist_pointer. entailer!.
-    refold_freelistrep. entailer.
-    rewrite kalloc_token'_split. Exists v. entailer. admit.
-+ forward. destruct (eq_dec original_freelist_pointer nullval) eqn:e1; auto_contradict. entailer.
-    rewrite mem_mgr_split. Exists sh ([]:list val) xx nullval. entailer!. destruct H0 as [[H011 H012]| [H021 H022]]; auto_contradict.
-    rewrite H011. entailer.
-+ destruct (eq_dec original_freelist_pointer nullval) eqn:e1. 
-    *forward. Exists nullval. entailer.
-    * forward. Exists original_freelist_pointer. entailer!. destruct (eq_dec original_freelist_pointer nullval) eqn:e2; auto_contradict.
+    forward. (*unfold abbreviate in POSTCONDITION.*) forward.
     entailer.
-Admitted. 
+    (*destruct (eq_dec original_freelist_pointer nullval) eqn:e1; auto_contradict. entailer.*)
+    rewrite mem_mgr_split. Intros. 
+    refold_freelistrep. if_tac.
+    * rewrite H11 in H0022; auto_contradict.
+    * entailer. Exists v ls. entailer. unfold my_kalloc_token.
+    rewrite kalloc_token_sz_split. rewrite mem_mgr_split. entailer!.
+    -- split. unfold malloc_compatible. destruct original_freelist_pointer; auto_contradict. 
+        unfold malloc_compatible in H3. destruct H3. split; auto.
+        try rep_lia.
+        destruct ls.
+        ++ left; split; auto. rewrite <- H9; auto.
+        ++ right. split.
+            **  unfold not. intros; auto_contradict.
+            ** rewrite <- H10. unfold not; intros; auto_contradict.
+    -- apply data_at_memory_block.
+-forward. destruct (eq_dec original_freelist_pointer nullval) eqn:e1; auto_contradict. entailer.
+rewrite mem_mgr_split. entailer.
+- if_tac; forward.
+Qed.
+
